examples/byte_register.thy
@@ -1,0 +1,118 @@
+(*
+This is the byte register example from Michael Banks's PhD thesis [On Confidentiality and Formal
+Methods] Section 3.4.3, page 37
+
+This is a register that stores a byte value and an error bit. It also defines a double operation
+which doubles the value in the register, if possible.
+*)
+
+theory byte_register
+  imports Main "../Banks/banks" (*NO_CI*)
+  (*CI_ONLY imports Main "Banks.banks" CI_ONLY*)
+begin
+
+alphabet \<alpha>ST = 
+  reg :: int
+  err :: int
+
+alphabet \<alpha>H =
+  reg\<^sub>H :: int
+  err\<^sub>H :: int
+
+alphabet \<alpha>L =
+  reg\<^sub>L :: int
+  err\<^sub>L :: int
+
+(* ST defines what states are valid *)
+definition ST
+  where "ST = (reg \<ge> 0 \<and> reg \<le> 255 \<and> err \<ge> 0 \<and> err \<le> 1)\<^sub>e"
+
+(* DBL doubles the number, if it is low enough to double without overflow *)
+definition DBL
+  where "DBL = Sys ((reg\<^sup>< \<ge> 0 \<and> reg\<^sup>< \<le> 127 \<and> err\<^sup>< = 0)\<^sub>e \<turnstile>\<^sub>r (reg\<^sup>> = reg\<^sup>< * 2 \<and> err\<^sup>> = 0)\<^sub>e)"
+
+(* A view of the high nibble *)
+definition Hv
+  where "Hv = OK (vu:\<^bold>v\<^sub>D:reg\<^sub>H = floor (sys:\<^bold>v\<^sub>D:reg / 16) \<and> vu:\<^bold>v\<^sub>D:err\<^sub>H = sys:\<^bold>v\<^sub>D:err)\<^sub>e"
+
+(* A view of the low nibble *)
+definition Lv
+  where "Lv = OK (vu:\<^bold>v\<^sub>D:reg\<^sub>L = sys:\<^bold>v\<^sub>D:reg mod 16 \<and> vu:\<^bold>v\<^sub>D:err\<^sub>L = sys:\<^bold>v\<^sub>D:err)\<^sub>e"
+
+(*
+Consider an example where the register stores the value 60
+
+60(b10) = 111100(b2)
+
+Here is an observation on the final state, with this value
+*)
+definition \<Phi> where "\<Phi> =  ((Sys1 ((reg = 60 \<and> err = 0)\<^sub>e \<up> \<^bold>v\<^sub>D))\<^sup>>)\<^sub>e"
+
+(*
+  Hv and Lv extract the high nibble and low nibble, respectively
+  ..111100(b2)
+  HHHH     = 11(b2)   = 3(b10)
+      LLLL = 1100(b2) = 12(b10)
+*)
+lemma "(L Hv \<Phi>) = ((Vu1 ((reg\<^sub>H = 3 \<and> err\<^sub>H = 0)\<^sub>e \<up> \<^bold>v\<^sub>D))\<^sup>>)\<^sub>e"
+  by (expr_simp_banks add: Hv_def \<Phi>_def)
+
+lemma "(L Lv \<Phi>) = ((Vu1 ((reg\<^sub>L = 12 \<and> err\<^sub>L = 0)\<^sub>e \<up> \<^bold>v\<^sub>D))\<^sup>>)\<^sub>e"
+  by (expr_simp_banks add: Lv_def \<Phi>_def)
+
+(* DBL2 doubles the number, if it is low enough to double without overflow, but unlike DBL, it
+explicitly defines the behaviour in the overflow case. If overflow is detected, then the err bit is
+set and the register contains an arbitrary value.*)
+definition DBL2
+  where "DBL2 = Sys (
+    (reg\<^sup>< \<ge> 0 \<and> reg\<^sup>< \<le> 255 \<and> err\<^sup>< = 0)\<^sub>e
+    \<turnstile>\<^sub>r
+    ((reg\<^sup>> = reg\<^sup>< * 2 \<and> err\<^sup>> = 0) \<lhd> (reg \<le> 127) \<rhd> (reg\<^sup>> \<ge> 0 \<and> reg\<^sup>> \<le> 255 \<and> err\<^sup>> = 0))\<^sub>e
+  )"
+
+(* DBL is refined by DBL2 *)
+lemma "DBL \<sqsubseteq> DBL2"
+  by (expr_simp_banks add: DBL_def DBL2_def, pred_auto)
+
+term Lv
+
+
+term "(reg\<^sub>L \<ge> 0 \<and> reg\<^sub>L \<le> 7 \<and> err\<^sub>L = 0)\<^sub>e"
+
+term "(((reg\<^sub>H\<^sup>> = (reg\<^sub>H\<^sup>< * 2)) \<or> (reg\<^sub>H\<^sup>> = ((reg\<^sub>H\<^sup>< * 2) + 1))) \<and> (err\<^sub>H\<^sup>> = 0))\<^sub>e"
+
+term "L (Hv \<and> Sys1 (ST \<up> \<^bold>v\<^sub>D)) DBL"
+
+term "L (Hv \<and> Sys1 (ST \<up> \<^bold>v\<^sub>D)) DBL"
+
+term "(((vu:\<^bold>v\<^sub>D:reg\<^sub>H\<^sup>> = (vu:v\<^sub>D:reg\<^sub>H\<^sup>< * 2)) \<or> (vu:v\<^sub>D:reg\<^sub>H\<^sup>> = ((vu:v\<^sub>D:reg\<^sub>H\<^sup>< * 2) + 1))) \<and> (vu:v\<^sub>D:err\<^sub>H\<^sup>> = 0))\<^sub>e"
+
+term "(Vu1 (reg\<^sub>H \<ge> 0 \<and> reg\<^sub>H \<le> 7 \<and> err\<^sub>H = 0)\<^sub>e)\<^sup><"
+term "
+  (Vu1 (\<^bold>v\<^sub>D:reg\<^sub>H \<ge> 0 \<and> \<^bold>v\<^sub>D:reg\<^sub>H \<le> 7 \<and> \<^bold>v\<^sub>D:err\<^sub>H = 0)\<^sub>e)\<^sup><
+  \<turnstile>\<^sub>r
+  (((vu:\<^bold>v\<^sub>D:reg\<^sub>H\<^sup>> = (vu:v\<^sub>D:reg\<^sub>H\<^sup>< * 2)) \<or> (vu:v\<^sub>D:reg\<^sub>H\<^sup>> = ((vu:v\<^sub>D:reg\<^sub>H\<^sup>< * 2) + 1))) \<and> (vu:v\<^sub>D:err\<^sub>H\<^sup>> = 0))\<^sub>e
+"
+
+term "(L (Hv \<and> Sys1 (ST \<up> \<^bold>v\<^sub>D)) DBL) =(
+  (reg\<^sub>H\<^sup>< \<ge> 0 \<and> reg\<^sub>H\<^sup>< \<le> 7 \<and> err\<^sub>H\<^sup>< = 0)\<^sub>e
+  \<turnstile>\<^sub>r
+  (((reg\<^sub>H\<^sup>> = (reg\<^sub>H\<^sup>< * 2)) \<or> (reg\<^sub>H\<^sup>> = ((reg\<^sub>H\<^sup>< * 2) + 1))) \<and> (err\<^sub>H\<^sup>> = 0))\<^sub>e)
+"
+
+
+term "(Sys1 (ST \<up> \<^bold>v\<^sub>D))\<^sup><"
+
+
+term "(Lv \<and> Sys1 (ST \<up> \<^bold>v\<^sub>D))"
+
+term "L (Lv \<and> Sys1 (ST \<up> \<^bold>v\<^sub>D)) DBL2"
+
+term "(reg\<^sub>L \<ge> 0 \<and> reg\<^sub>L \<le> 15 \<and> err\<^sub>L = 0)\<^sub>e"
+
+term "((reg\<^sub>L\<^sup>> = (reg\<^sub>L\<^sup>< * 2) mod 16 \<and> err\<^sub>L\<^sup>> = 0) \<or> (reg\<^sub>L\<^sup>> \<ge> 0 \<and> reg\<^sub>L\<^sup>> \<le> 15 \<and> err\<^sub>L\<^sup>> = 1))\<^sub>e"
+
+
+lemma "L (Lv \<and> Sys1 (ST \<up> \<^bold>v\<^sub>D)) DBL2"
+
+end
